import nuclear reactor (mathlib)

ConcreteSemanticsLean/ch2.lean
@@ -1,30 +1,34 @@
 import ConcreteSemanticsLean.cslib
 import Init.Prelude
+import Mathlib.Tactic.Linarith
 
 -- 2.1
 
 -- 2.2
 
 -- 2.3
-def count [DecidableEq X] (elm : X) (l : mylist X) (occ : Nat) : Nat :=
+def count [DecidableEq X] (elm : X) (l : mylist X) : Nat :=
   match l with
-  | [] => occ
-  | a :: l' => if elm = a then count elm l' (occ + 1) else count elm l' occ
+  | [] => 0
+  | a :: l' => if elm = a then 1 + count elm l' else count elm l'
 
-#eval count 1 (1 :: 2 :: 1 :: []) 0 -- 2
-#eval count 3 (1 :: 2 :: 1 :: []) 0 -- 0
-#eval count type1.A type1_list 0 -- 1
+#eval count 1 (1 :: 2 :: 1 :: []) -- 2
+#eval count 3 (1 :: 2 :: 1 :: []) -- 0
+#eval count type1.A type1_list -- 1
 
 -- someone should try to find  way to remove the need for DecidableEq
-theorem count_x_le_len [DecidableEq X] : ∀ (elm : X) (l : mylist X), count elm l 0 ≤ len l := by
+theorem count_x_le_len [DecidableEq X] : ∀ (elm : X) (l : mylist X), count elm l ≤ len l := by
   intros elm l
   induction l
-  . simp [count, len]
-  . simp [count, len]
-    sorry
-
-
-
+  case nil =>
+    simp [count, len]
+  case cons head tl ih =>
+    simp [count, len]  -- Simplify count and len for the cons case
+    by_cases h : elm = head
+    -- Case when elm = hd
+    . simp [h]; rw [← h]; exact ih
+   -- Case when elm ≠ hd
+    . simp [h]; linarith
 
 
 -- 2.4
